WIP

code/ecdsa/Hacl.Impl.EC.Core.fst
@@ -150,7 +150,7 @@ val normalisation_update: #c: curve -> z2x: felem c -> z3y: felem c -> p: point 
     let x1, y1, z1 = point_as_nat c h1 resultPoint in
     x1 == fromDomain_ #c #DH (as_nat c h0 z2x) /\ 
     y1 == fromDomain_ #c #DH (as_nat c h0 z3y) /\ (
-    if Spec.ECC.isPointAtInfinity #c #Jacobian (fromDomain_ #c #DH x0, fromDomain_ #c #DH y0, fromDomain_ #c #DH z0) 
+    if Spec.ECC.isPointAtInfinity #Jacobian (fromDomain_ #c #DH x0, fromDomain_ #c #DH y0, fromDomain_ #c #DH z0) 
     then z1 == 0 else z1 == 1)))
 
 let normalisation_update #c z2x z3y p resultPoint = 
@@ -181,7 +181,7 @@ val lemma_norm: #c: curve -> pD : point_nat_prime #c -> r: point_nat_prime #c ->
     let x3, y3, z3 = r in 
     x3 == xD * (pow (zD * zD % prime) (prime - 2) % prime) % prime /\
     y3 == yD * (pow ((zD * zD % prime) * zD % prime) (prime - 2) % prime) % prime/\
-    (if Spec.ECC.isPointAtInfinity #c #Jacobian (xD, yD, zD) then z3 == 0 else z3 == 1)))
+    (if Spec.ECC.isPointAtInfinity #Jacobian (xD, yD, zD) then z3 == 0 else z3 == 1)))
   (ensures (let xN, yN, zN = _norm #c pD in r == (xN, yN, zN))) 
 
 
@@ -352,12 +352,12 @@ inline_for_extraction noextract
 val uploadStartPoints: #c: curve -> q: point c -> p: point c -> result: point c -> Stack unit 
   (requires fun h -> live h q /\ live h p /\ live h result /\
     disjoint p q /\ disjoint q result /\ eq_or_disjoint p result /\ point_eval c h p /\
-    ~ (isPointAtInfinity  #c #Jacobian (point_as_nat c h p)))
+    ~ (isPointAtInfinity #Jacobian (point_as_nat c h p)))
   (ensures fun h0 _ h1 -> modifies (loc result |+| loc q) h0 h1 /\
     point_eval c h1 q /\ point_eval c h1 result /\ (
     let pD = fromDomainPoint #c #DH (point_as_nat c h1 q) in 
     let qD = fromDomainPoint #c #DH (point_as_nat c h1 result) in 
-    qD == point_as_nat c h0 p /\ isPointAtInfinity #c pD /\ 
+    qD == point_as_nat c h0 p /\ isPointAtInfinity pD /\ 
     pointEqual #c pD (point_mult #c 0 qD) /\ ~ (pointEqual #c pD qD)))
 
 let uploadStartPoints #c q p result = 
@@ -389,7 +389,7 @@ val scalar_multiplication_t_0: #c: curve -> #t:buftype -> #l : ladder
   (requires fun h ->  live h p /\ live h result /\ live h scalar /\ live h tempBuffer /\
     LowStar.Monotonic.Buffer.all_disjoint [loc p;  loc tempBuffer; loc scalar] /\
     eq_or_disjoint p result /\ disjoint result tempBuffer /\ disjoint result scalar /\
-    point_eval c h p /\ ~ (isPointAtInfinity #c #Jacobian (point_as_nat c h p)) /\
+    point_eval c h p /\ ~ (isPointAtInfinity #Jacobian (point_as_nat c h p)) /\
     scalar_as_nat (as_seq h scalar) < getOrder #c)
   (ensures fun h0 _ h1 -> modifies (loc result |+| loc tempBuffer) h0 h1 /\ point_eval c h1 result /\ (
     let p0 = point_as_nat c h0 p in 
@@ -462,7 +462,7 @@ val scalarMultiplication_t: #c: curve -> #t:buftype -> #l: ladder -> p: point c 
     live h p /\ live h result /\ live h scalar /\ live h tempBuffer /\
     scalar_as_nat (as_seq h scalar) < getOrder #c /\ 
     LowStar.Monotonic.Buffer.all_disjoint [loc p; loc tempBuffer; loc scalar; loc result] /\ point_eval c h p /\
-    ~ (isPointAtInfinity #c #Jacobian (point_as_nat c h p)))
+    ~ (isPointAtInfinity #Jacobian (point_as_nat c h p)))
   (ensures fun h0 _ h1 -> modifies (loc p |+| loc result |+| loc tempBuffer) h0 h1 /\ point_eval c h1 result /\ (
     let p0 = point_as_nat c h0 p in 
     let qD = point_as_nat c h1 result in
@@ -529,7 +529,7 @@ val uploadStartPointsS2P: #c: curve -> q: point c -> result: point c -> Stack un
     point_eval c h1 q /\ point_eval c h1 result /\ (
     let pD = fromDomainPoint #c #DH (point_as_nat c h1 q) in 
     let qD = fromDomainPoint #c #DH (point_as_nat c h1 result) in 
-    qD == basePoint #c /\ pD == pointAtInfinity #c /\ 
+    qD == basePoint #c /\ isPointAtInfinity pD /\ 
     pointEqual #c pD (point_mult #c 0 qD) /\ ~ (pointEqual #c pD qD)))
 
 let uploadStartPointsS2P #c q result = 
@@ -556,14 +556,15 @@ let secretToPublic #c #l result scalar tempBuffer =
       uploadStartPointsS2P q result; 
       montgomery_ladder q result scalar buff;
 	let h1 = ST.get() in 
-      norm q result buff;   
-	norm_twice_lemma #c (fromDomainPoint #c #DH (point_as_nat c h1 q)) (point_mult #c (scalar_as_nat #c (as_seq h0 scalar)) (basePoint #c))
+      norm q result buff;
+      norm_twice_lemma #c (fromDomainPoint #c #DH (point_as_nat c h1 q)) (point_mult #c (scalar_as_nat #c (as_seq h0 scalar)) (basePoint #c))
     end
   |Radix  -> 
     begin
-      admit();
       secret_to_public_radix q scalar buff;
-      norm q result buff
+	let h1 = ST.get() in 
+      norm q result buff;
+      norm_twice_lemma #c (fromDomainPoint #c #DH (point_as_nat c h1 q)) (point_mult #c (scalar_as_nat #c (as_seq h0 scalar)) (basePoint #c))
     end
 
 
@@ -572,13 +573,12 @@ val secretToPublicWithoutNorm_: #c: curve -> #l: ladder -> result: point c
   -> scalar: scalar_t #MUT #c
   -> tempBuffer: lbuffer uint64 (size 20 *! getCoordinateLenU64 c) ->
   Stack unit (requires fun h -> live h result /\ live h scalar /\ live h tempBuffer /\ 
-    LowStar.Monotonic.Buffer.all_disjoint [loc tempBuffer; loc scalar; loc result])
+    LowStar.Monotonic.Buffer.all_disjoint [loc tempBuffer; loc scalar; loc result] /\ 
+    scalar_as_nat (as_seq h scalar) < getOrder #c)
   (ensures fun h0 _ h1 -> point_eval c h1 result /\ modifies (loc result |+| loc tempBuffer) h0 h1 /\ (
     let p0 = basePoint #c in 
     let qD = fromDomainPoint #c #DH (point_as_nat c h1 result) in
-    pointEqual #c qD (point_mult #c (scalar_as_nat #c (as_seq h0 scalar)) p0) /\
-    pointEqual #c qD (secret_to_public (as_seq h0 scalar))))
-
+    pointEqual #c qD (point_mult #c (scalar_as_nat #c (as_seq h0 scalar)) p0)))
 
 let secretToPublicWithoutNorm_ #c #l result scalar tempBuffer = 
   let h0 = ST.get() in 
@@ -594,8 +594,7 @@ let secretToPublicWithoutNorm_ #c #l result scalar tempBuffer =
     end
   |Radix  -> 
     begin
-      admit();
-      secret_to_public_radix q scalar buff
+      secret_to_public_radix result scalar buff
     end
 
 
