specs/ecdsa/Spec.ECC.Radix.fst
@@ -21,19 +21,6 @@ open Spec.ECC
 
 let radix = 4
 
-
-val toAffine: #c: curve -> #coordSystem : coordSyst -> p: point #c #coordSystem -> point #c #Affine
-
-let toAffine #c #coordSystem p = 
-  match coordSystem with 
-  |Affine -> p
-  |Jacobian -> 
-    if isPointAtInfinity p then 
-      pointAtInfinity #c #Affine 
-    else
-      let pNormX, pNormY, pNormZ = _norm #c p in 
-      (pNormX, pNormY)
-
 val lemma_is_point_on_curve: #c: curve -> p: point #c #Jacobian {~ (isPointAtInfinity p) /\ pointOnCurve #c p} 
   -> Lemma (
     let pX, pY, pZ = p in 
@@ -49,77 +36,6 @@ let lemma_is_point_on_curve #c p =
       assert(	0 == bCoordinate #c);
       assert(False)
     end
-
-
-val lemma_toAffine_fromAffine: #c: curve -> p: point #c #Jacobian {isPointAtInfinity p \/ pointOnCurve #c p} -> Lemma (
-  let pA = toAffine p in 
-  let pAJ = toJacobianCoordinates pA in 
-  pointEqual pAJ p)
-
-let lemma_toAffine_fromAffine #c p = 
-  let pAx, pAy = toAffine p in 
-  let pAJ = toJacobianCoordinates #c (pAx, pAy) in 
-
-  if isPointAtInfinity p then () else begin
-    let x, y, z = p in 
-    
-    assert(pAx == (modp_inv2 #c (z * z) * x) % getPrime c);
-    assert(pAy == (modp_inv2 #c (z * z * z) * y) % getPrime c);
-    assert(z <> 0);
-
-    lemma_is_point_on_curve #c p;
-    
-    assume (pAx <> 0 \/ pAy <> 0);
-    
-    assume (
-      let pAffineX, pAffineY, pAffineZ = _norm p in 
-      let qAffineX, qAffineY, qAffineZ = _norm #c (_norm p) in 
-
-      pAffineX = qAffineX && pAffineY = qAffineY);
-
-
-    assert (pointEqual (pAx, pAy, 1) p)
-  end
-
-
-val getPrecomputedPoint_Affine: #c: curve -> p: point #c #Jacobian -> i: nat {i < 16} -> 
-  Tot (r: point #c #Affine {
-    pointEqual (toJacobianCoordinates r) (point_mult #c i p) /\ (
-    if i = 0 then isPointAtInfinity #c #Affine r 
-    else 
-      isPointAtInfinity #c #Affine r == false)})
-
-let getPrecomputedPoint_Affine #c p i = 
-  let r : point #c #Affine = 
-    if i = 0 then 
-      begin
-      	point_mult_0 #c p i;
-	pointAtInfinity #c #Affine
-      end
-    else begin
-      let r = toAffine (point_mult #c i p) in 
-      assume (isPointAtInfinity #c #Affine r == false);
-      r
-    end in 
-  assume (pointOnCurve (point_mult #c i p));
-  lemma_toAffine_fromAffine (point_mult #c i p);
-  r
-
-
-val getPrecomputedPoint_Jacobian: #c: curve -> p: point #c #Jacobian -> i: nat -> 
-  Tot (r: point #c #Jacobian {pointEqual r (point_mult #c i p)})
-
-let getPrecomputedPoint_Jacobian #c p i = 
-  point_mult #c i p
- 
-
-val getPrecomputedPoint: #c: curve -> #t: coordSyst -> p: point #c #Jacobian -> i: nat {i < 16} -> 
-  Tot (r: point #c #Jacobian {pointEqual r (point_mult #c i p)})
-
-let getPrecomputedPoint #c #t p i = 
-  match t with 
-  |Affine -> toJacobianCoordinates (getPrecomputedPoint_Affine #c p i)
-  |Jacobian -> getPrecomputedPoint_Jacobian #c p i
 
 
 val repeatAsDoubling: #c: curve -> p: point #c #Jacobian -> i: nat -> Lemma (
@@ -166,12 +82,12 @@ let radix_step #c #t k p0 i p =
   let l = v (getScalarLen c) in 
   let si = arithmetic_shift_right scalar (l - (i + 2) * radix) % pow2 radix in 
   let pRadixed = getPointDoubleNTimes #c p radix in 
-  let pointPrecomputed = getPrecomputedPoint #c #t p0 si in 
+  let pointPrecomputed = point_mult #c si p0 in 
   pointAdd #c pRadixed pointPrecomputed
 
 val lemmaIsPointAtInf: #c: curve ->  q: point_nat_prime #c  ->
   Lemma (requires  (let x, y, z = q in z == 0))
-  (ensures isPointAtInfinity #c #Jacobian q)
+  (ensures isPointAtInfinity  #Jacobian q)
 
 let lemmaIsPointAtInf #c q = ()
 
@@ -179,8 +95,8 @@ let lemmaIsPointAtInf #c q = ()
 #push-options " --ifuel 1"
 
 val pointAddDoubleWithTwoPointInfinity: #c: curve -> 
-  q: point_nat_prime #c {isPointAtInfinity #c #Jacobian q} ->
-  r: point_nat_prime #c {isPointAtInfinity #c #Jacobian r} -> 
+  q: point_nat_prime #c {isPointAtInfinity #Jacobian q} ->
+  r: point_nat_prime #c {isPointAtInfinity  #Jacobian r} -> 
   Lemma (pointEqual (_point_add #c q r) (pointAdd #c  q r))
 
 let pointAddDoubleWithTwoPointInfinity #c q r = 
@@ -195,51 +111,6 @@ val curve_distributivity: #c: curve -> p0: point_nat_prime #c
   -> Lemma (pointEqual q (point_mult #c (a % getOrder #c) p0))
 
 let curve_distributivity #c p0 a q = lemma_scalar_reduce #c p0 a
-
-val pointAddNotEqual: #c: curve ->
-  p0: point_nat_prime #c ->
-  b: nat -> 
-  r: point_nat_prime #c {pointEqual r (point_mult #c b p0)} ->
-  a: nat -> 
-  q: point_nat_prime #c {pointEqual q (point_mult #c a p0)} -> 
-  Lemma 
-  (requires ((a < b \/ isPointAtInfinity #c #Jacobian r) /\ a < getOrder #c))
-  (ensures (
-    if isPointAtInfinity #c #Jacobian q && isPointAtInfinity #c #Jacobian  r then 
-      pointEqual (_point_add #c q r) (pointAdd #c  q r) 
-    else 
-      ~ (pointEqual #c q r) /\ ~ (pointEqual #c r q)) )
-  
-
-let pointAddNotEqual #c p0 b r a q = 
-  admit(); 
-  if isPointAtInfinity #c #Jacobian q && isPointAtInfinity #c #Jacobian r then 
-    pointAddDoubleWithTwoPointInfinity q r
-  else if isPointAtInfinity #c #Jacobian q then ()
-  else if isPointAtInfinity #c #Jacobian r then () 
-  else begin
-    let order = getOrder #c in 
-    let aPrime = getOrder #c - a in 
-    let qPrime = point_mult #c  aPrime p0 in 
-    let aQprime = pointAdd #c  q qPrime in 
-    lemmaApplPointAdd #c p0 a q aPrime qPrime;
-    point_mult_0 #c  p0 (a + aPrime);
-
-  if (aPrime + b < order) then 
-    begin
-      curve_order_is_the_smallest #c  p0;
-      assert(~ (isPointAtInfinity #c #Jacobian (point_mult #c (aPrime + b) p0)));
-      assert(~ (pointEqual #c q r))
-    end
-  else 
-    begin
-      assert(aPrime + b >= order);
-      assert(a < b);
-      curve_distributivity p0 (aPrime + b) (point_mult #c (aPrime + b) p0);
-      assert(pointEqual (point_mult #c  (aPrime + b) p0) (point_mult #c  ((aPrime + b) % order) p0));
-      curve_order_is_the_smallest #c  p0
-    end
-  end
 
 
 val curve_multiplication_distributivity: 
@@ -265,6 +136,7 @@ let rec curve_multiplication_distributivity #c p0 a q b r =
 
     curve_compatibility_with_translation_lemma #c  q (point_mult #c  a p0) a_1;
     assert(pointEqual (pointAdd #c  q a_1) (pointAdd #c  (point_mult #c  a p0) a_1));
+  
     lemmaApplPointAdd #c  p0 a (point_mult #c  a p0) (a * (b - 1)) a_1;
 
     let open FStar.Tactics in 
@@ -307,7 +179,7 @@ let pred0 #c #t x s p0 i =
   if pointEqual x (point_mult #c partialScalar p0) then begin
     let si = arithmetic_shift_right scalar (l - (i + 2) * radix) % pow2 radix in 
     let pRadixed = getPointDoubleNTimes x radix in 
-    let pointPrecomputed = getPrecomputedPoint #c #t p0 si in 
+    let pointPrecomputed = point_mult #c si p0 in 
     let p = pointAdd #c pRadixed pointPrecomputed in
     curve_multiplication_distributivity #c p0 partialScalar x (pow2 radix) pRadixed;
     if si > 0 && partialScalar > 0 then
@@ -317,26 +189,26 @@ let pred0 #c #t x s p0 i =
       if si = 0 then 
 	if partialScalar = 0 then begin
 	  point_mult_0 #c p0 0;
-	  assert(isPointAtInfinity #c pointPrecomputed /\ isPointAtInfinity #c #Jacobian pRadixed) end
+	  assert(isPointAtInfinity  pointPrecomputed /\ isPointAtInfinity #Jacobian pRadixed) end
 	else 
 	  assert(si < b)
       else
 	begin
 	  assert(partialScalar = 0);
 	  point_mult_0 #c p0 0;
-	  assert(isPointAtInfinity #c #Jacobian pRadixed)
+	  assert(isPointAtInfinity #Jacobian pRadixed)
 	end 
   end;
-
+  
   begin match t with
     |Affine ->
       if si = 0 then begin
-	assert(pointEqual pRadixed (point_mult (pow2 radix) x));
+	assert(pointEqual pRadixed (point_mult (pow2 radix) x)); 
 	assert(p == pointAdd pRadixed pointPrecomputed);
-	assert(si == 0);
+	assert(pointPrecomputed == point_mult #c si p0);
 
-	assert(pointPrecomputed == getPrecomputedPoint #c #t p0 si); 
-	assert(isPointAtInfinity #c pointPrecomputed);
+	point_mult_0 p0 si;
+	assert(isPointAtInfinity  pointPrecomputed);
 	
 	curve_point_at_infinity_property #c pRadixed;
 	curve_commutativity_lemma #c pRadixed pointPrecomputed;
@@ -345,13 +217,15 @@ let pred0 #c #t x s p0 i =
       else begin
 	assert(pointEqual pRadixed (point_mult (pow2 radix) x));
 	assert(p == pointAdd pRadixed pointPrecomputed);
-	assert(pointPrecomputed == toJacobianCoordinates (getPrecomputedPoint #c #t p0 si));
-
+	assert(pointPrecomputed == toJacobianCoordinates (point_mult #c si p0));
+	
 	assert(pointEqual p (pointAdd pRadixed pointPrecomputed));
-	
-	pointAddNotEqual p0 b pRadixed si (toJacobianCoordinates pointPrecomputed);
-	
-	lemmaApplPointAdd #c p0 (pow2 radix * partialScalar) pRadixed si (toJacobianCoordinates (getPrecomputedPoint #c #t p0 si));
+
+
+	assert (pointEqual pRadixed (point_mult (pow2 radix * partialScalar) p0));
+	assert (pointEqual (toJacobianCoordinates (point_mult #c si p0)) (point_mult si p0));
+
+	lemmaApplPointAdd #c p0 (pow2 radix * partialScalar) pRadixed si (toJacobianCoordinates (point_mult #c si p0));
 
 	(* C == A *)
       	assert(pointEqual p (pointAdd pRadixed pointPrecomputed));
@@ -362,10 +236,10 @@ let pred0 #c #t x s p0 i =
 	assert(pointEqual p (point_mult (pow2 radix * partialScalar + si) p0))
       end
     |Jacobian -> 
-	pointAddNotEqual p0 b pRadixed si pointPrecomputed;
 	lemmaApplPointAdd #c p0 (pow2 radix * partialScalar) pRadixed si pointPrecomputed;
 	curve_commutativity_lemma #c pRadixed pointPrecomputed;
 	assert(pointEqual p (point_mult (si + pow2 radix * partialScalar) p0)) end;
+	
     lemma_div_mod (div scalar (pow2 (l - (i + 2) * radix))) (pow2 radix);
     division_multiplication_lemma scalar (pow2 (l - (i + 2) * radix)) (pow2 radix);
     pow2_plus (l - (i + 2) * radix) radix
@@ -401,8 +275,7 @@ let radix_spec #c #t s p0 =
   let l = v (getScalarLen c) in  
     scalar_as_nat_upperbound s l;
     lemma_div_lt_nat scalarNat l radix;
-  let pointToStart = toJacobianCoordinates 
-    (getPrecomputedPoint #c #t p0 (arithmetic_shift_right scalarNat (l - radix))) in  
+  let pointToStart = toJacobianCoordinates (point_mult (arithmetic_shift_right scalarNat (l - radix)) p0) in  
 
   let len = (l / radix) - 1 in 
   let pred (i: nat {i <= len}) (p : point #c #Jacobian) : Type0 = (
