code/ecdsa/Hacl.Impl.EC.PointAddC.fsti
@@ -29,8 +29,8 @@ inline_for_extraction noextract
 val point_add_c_out: #c: curve -> p: point c -> q: point c -> result: point c ->
   Stack unit (requires fun h -> live h p /\ live h q /\ live h result /\ 
     eq_or_disjoint q result /\ disjoint p q /\ disjoint p result /\
-     point_eval c h p /\ point_eval c h q /\ ~ (isPointAtInfinity #c #Jacobian (point_as_nat c h p)) /\ 
-     ~ (isPointAtInfinity #c #Jacobian (point_as_nat c h q)))
+     point_eval c h p /\ point_eval c h q /\ ~ (isPointAtInfinity #Jacobian (point_as_nat c h p)) /\ 
+     ~ (isPointAtInfinity #Jacobian (point_as_nat c h q)))
    (ensures fun h0 _ h1 -> modifies (loc result) h0 h1 /\ point_eval c h1 result /\ (
      let pD = fromDomainPoint #c #DH (point_as_nat c h0 p) in 
      let qD = fromDomainPoint #c #DH (point_as_nat c h0 q) in 
