code/ecdsa/Hacl.Impl.EC.PointAddMixed.fsti
@@ -26,6 +26,6 @@ val point_add_mixed: #c: curve -> p: point c -> q: pointAffine c -> result: poin
     disjoint q tempBuffer /\ disjoint q result /\ disjoint result tempBuffer /\  
     point_eval c h p /\ point_aff_eval c h q)
   (ensures fun h0 _ h1 -> modifies (loc tempBuffer |+| loc result) h0 h1 /\ point_eval c h1 result /\ (
-    let qD = fromDomainPoint #c #DH (toJacobianCoordinates #c (point_affine_as_nat c h0 q)) in 
+    let qD = fromDomainPoint #c #DH (toJacobianCoordinates (point_affine_as_nat c h0 q)) in 
     fromDomainPoint #c #DH (point_as_nat c h1 result) == 
     _point_add #c  (fromDomainPoint #c #DH (point_as_nat c h0 p)) qD))
