code/ecdsa/Hacl.Impl.P256.Signature.Common.fst
@@ -112,7 +112,7 @@ val toFormPoint_: #c: curve -> i: pointAffine8 c -> o: point c -> Stack unit
     let pointScalarXSeq = nat_from_bytes_be (as_seq h0 (getXAff8 i))  in 
     let pointScalarYSeq = nat_from_bytes_be (as_seq h0 (getYAff8 i)) in 
     let x, y, z = as_nat c h1 (getX o), as_nat c h1 (getY o), as_nat c h1 (getZ o) in  
-    let pointJacX, pointJacY, pointJacZ = toJacobianCoordinates #c (pointScalarXSeq, pointScalarYSeq) in 
+    let pointJacX, pointJacY, pointJacZ = toJacobianCoordinates (pointScalarXSeq, pointScalarYSeq) in 
     x == pointScalarXSeq /\ y == pointScalarYSeq /\ z == 1 /\
     x == pointJacX /\ y == pointJacY /\ z == pointJacZ))
       
